fix: bug with constraint generation

Grw/Morphism.lean
@@ -398,3 +398,51 @@ theorem properOrIff: Proper (Iff ⟹ Iff ⟹ Iff) Or :=
 @[grewrite]
 theorem properNotIff: Proper (Iff ⟹ Iff) Not :=
   ⟨fun _ _ h => by simp [h]⟩
+
+def setEq : List α → List α → Prop :=
+  fun l1 l2 => ∀ x, x ∈ l1 <-> x ∈ l2
+
+instance setEqEquivalence {α : Type} : Equivalence (@setEq α) where
+  refl := fun l1 x => Iff.rfl  -- Reflexivity: l1 ≈ l1
+  symm := by  -- Symmetry: If l1 ≈ l2, then l2 ≈ l1
+    intro x y hxy
+    unfold setEq
+    intro a
+    apply Iff.symm
+    exact hxy a
+  trans := by
+    intro x y z hxy hyz
+    unfold setEq at *
+    intro a
+    apply Iff.intro
+    intro hx
+    rw [hxy a] at hx
+    rw [hyz a] at hx
+    assumption
+    intro hy
+    rw [← hyz a] at hy
+    rw [← hxy a] at hy
+    assumption
+
+def addElem {α : Type} (x : α) (l : List α) : List α :=
+  x :: l
+
+@[grewrite]
+theorem addElemProper {α : Type} (x : α) : @Proper (List α → List α) (setEq ⟹ setEq) (addElem x) := by
+  constructor
+  unfold respectful
+  intro l1 l2 heq x
+  simp [addElem]
+  constructor
+  · intro hx
+    cases hx with
+    | inl => left; assumption
+    | inr h' =>
+      right; exact (heq x).mp h'
+  · intro hx
+    cases hx with
+    | inl => left; assumption
+    | inr h' => right; exact (heq x).mpr h'
+
+initialize
+  Lean.registerTraceClass `Meta.Tactic.grewrite
